Kami/Ex/ProcDecInl.v
@@ -7,7 +7,7 @@ Set Implicit Arguments.
 Section Inlined.
   Variables addrSize iaddrSize fifoSize instBytes dataBytes rfIdx: nat.
 
-  Variables (fetch: AbsFetch instBytes dataBytes)
+  Variables (fetch: AbsFetch addrSize iaddrSize instBytes dataBytes)
             (dec: AbsDec addrSize instBytes dataBytes rfIdx)
             (exec: AbsExec iaddrSize instBytes dataBytes rfIdx).
 
