Kami/Ex/ProcFDInl.v
@@ -8,7 +8,7 @@ Set Implicit Arguments.
 Section Inlined.
   Variables addrSize iaddrSize instBytes dataBytes rfIdx: nat.
 
-  Variables (fetch: AbsFetch instBytes dataBytes)
+  Variables (fetch: AbsFetch addrSize iaddrSize instBytes dataBytes)
             (dec: AbsDec addrSize instBytes dataBytes rfIdx).
 
   Variable predictNextPc: forall ty, fullType ty (SyntaxKind (Pc iaddrSize)) -> (* pc *)
