Kami/Ex/ProcFetch.v
@@ -10,7 +10,7 @@ Set Implicit Arguments.
 Section FetchICache.
   Variables addrSize iaddrSize instBytes dataBytes rfIdx: nat.
 
-  Variables (fetch: AbsFetch instBytes dataBytes)
+  Variables (fetch: AbsFetch addrSize iaddrSize instBytes dataBytes)
             (predictNextPc:
                forall ty, fullType ty (SyntaxKind (Pc iaddrSize)) -> (* pc *)
                           Expr ty (SyntaxKind (Pc iaddrSize))).
@@ -75,7 +75,7 @@ Section FetchICache.
       Read pinitRqOfs : Bit iaddrSize <- "pinitRqOfs";
       Assert ((UniBit (Inv _) #pinitRqOfs) != $0);
 
-      Call memReq(STRUCT { "addr" ::= (_zeroExtend_ #pinitRqOfs) << $$(natToWord 2 2);
+      Call memReq(STRUCT { "addr" ::= alignAddr _ pinitRqOfs;
                            "op" ::= $$false;
                            "data" ::= $$Default });
       Write "pinitRqOfs" <- #pinitRqOfs + $1;
@@ -88,7 +88,7 @@ Section FetchICache.
       Assert !#pinitRq;
       Read pinitRqOfs : Bit iaddrSize <- "pinitRqOfs";
       Assert ((UniBit (Inv _) #pinitRqOfs) == $0);
-      Call memReq(STRUCT { "addr" ::= (_zeroExtend_ #pinitRqOfs) << $$(natToWord 2 2);
+      Call memReq(STRUCT { "addr" ::= alignAddr _ pinitRqOfs;
                            "op" ::= $$false;
                            "data" ::= $$Default });
       Write "pinitRq" <- $$true;
@@ -181,7 +181,7 @@ Hint Unfold instRq instRs
 Section Facts.
   Variables addrSize iaddrSize instBytes dataBytes rfIdx: nat.
 
-  Variables (fetch: AbsFetch instBytes dataBytes)
+  Variables (fetch: AbsFetch addrSize iaddrSize instBytes dataBytes)
             (predictNextPc:
                forall ty, fullType ty (SyntaxKind (Pc iaddrSize)) -> (* pc *)
                           Expr ty (SyntaxKind (Pc iaddrSize))).
@@ -219,13 +219,13 @@ Section Facts.
                           Expr ty (SyntaxKind Bool)).
 
   Lemma fetcher_ModEquiv:
-    forall pcInit, ModPhoasWf (fetcher addrSize fetch predictNextPc f2dPack pcInit).
+    forall pcInit, ModPhoasWf (fetcher fetch predictNextPc f2dPack pcInit).
   Proof. kequiv. Qed.
   Hint Resolve fetcher_ModEquiv.
 
   Lemma fetchICache_ModEquiv:
     forall pcInit,
-      ModPhoasWf (fetchICache addrSize fetch predictNextPc f2dPack pcInit).
+      ModPhoasWf (fetchICache fetch predictNextPc f2dPack pcInit).
   Proof.
     kequiv.
   Qed.
